coq: (WIP) structs

Primitives.v
@@ -1,6 +1,6 @@
-Require Export SGA.Common SGA.Types.
+Require Export SGA.Common SGA.Environments SGA.Types.
 
-Inductive prim_ufn_t :=
+Inductive prim_bits_ufn_t :=
 | USel
 | UPart (width: nat)
 | UAnd
@@ -14,7 +14,13 @@ Inductive prim_ufn_t :=
 | UZExtL (nzeroes: nat)
 | UZExtR (nzeroes: nat).
 
-Inductive prim_fn_t :=
+Inductive prim_struct_op := Init | Get | Put.
+
+Inductive prim_ufn_t :=
+| BitsUFn (fn: prim_bits_ufn_t)
+| StructUFn (op: prim_struct_op) (sig: struct_sig) (f: string).
+
+Inductive prim_bits_fn_t :=
 | Sel (sz: nat)
 | Part (sz: nat) (width: nat)
 | And (sz: nat)
@@ -27,6 +33,10 @@ Inductive prim_fn_t :=
 | UIntPlus (sz : nat)
 | ZExtL (sz: nat) (nzeroes: nat)
 | ZExtR (sz: nat) (nzeroes: nat).
+
+Inductive prim_fn_t :=
+| BitsFn (fn: prim_bits_fn_t)
+| StructFn (fn: prim_struct_op) (sig: struct_sig) (idx: Vect.index sig.(sv_len)).
 
 (* Like Nat.log2_iter, but switches to next power of two one number earlier
    (computes ceil(log2(n)) instead of floor(log2(n))). *)
@@ -42,6 +52,80 @@ Fixpoint log2_iter k_fuel p_logn q_n r_buffer :=
 
 Definition log2 n := log2_iter (pred n) 0 1 0.
 
+Fixpoint Vector_find {K: Type} {n: nat} {EQ: EqDec K} (k: K) (v: Vector.t K n) {struct n} : option (Vect.index n).
+Proof.
+  destruct n.
+  - exact None.
+  - destruct (eq_dec k (Vector.hd v)).
+    + exact (Some thisone).
+    + destruct (Vector_find K n EQ k (Vector.tl v)).
+      * exact (Some (anotherone i)).
+      * exact None.
+Defined.
+
+Fixpoint Vector_assoc {K V: Type} {n: nat} {EQ: EqDec K} (k: K) (v: Vector.t (K * V) n) {struct n} : option (Vect.index n).
+Proof.
+  destruct n.
+  - exact None.
+  - destruct (eq_dec k (fst (Vector.hd v))).
+    + exact (Some thisone).
+    + destruct (Vector_assoc K V n EQ k (Vector.tl v)).
+      * exact (Some (anotherone i)).
+      * exact None.
+Defined.
+
+Definition prim_uSigma (fn: prim_ufn_t) (tau1 tau2: type): result prim_fn_t fn_tc_error :=
+  match fn with
+  | BitsUFn fn =>
+    let/res sz1 := assert_bits_t tau1 in
+    let/res sz2 := assert_bits_t tau1 in
+    Success (BitsFn match fn with
+                    | USel => Sel sz1
+                    | UPart width => Part sz1 width
+                    | UAnd => And sz1
+                    | UOr => Or sz1
+                    | UNot => Not sz1
+                    | ULsl => Lsl sz1 sz2
+                    | ULsr => Lsr sz1 sz2
+                    | UEq => Eq sz1
+                    | UConcat => Concat sz1 sz2
+                    | UUIntPlus => UIntPlus sz1
+                    | UZExtL nzeroes => ZExtL sz1 nzeroes
+                    | UZExtR nzeroes => ZExtR sz1 nzeroes
+                    end)
+  | StructUFn op sig f =>
+    let/res idx := opt_result (Vector_assoc f sig.(sv_data)) (unbound_field f sig) in
+    Success (StructFn op sig idx)
+  end.
+
+Fixpoint Vector_nth {K: Type} {n: nat} (v: Vector.t K n) (idx: Vect.index n) {struct n} : K.
+Proof.
+  destruct n; destruct idx.
+  - exact (Vector.hd v).
+  - exact (Vector_nth K n (Vector.tl v) a).
+Defined.
+
+Definition prim_Sigma (fn: prim_fn_t) : ExternalSignature :=
+  match fn with
+  | BitsFn fn =>
+    match fn with
+    | Sel sz => {{ bits_t sz ~> bits_t (log2 sz) ~> bits_t 1 }}
+    | Part sz width => {{ bits_t sz ~> bits_t (log2 sz) ~> bits_t width }}
+    | And sz => {{ bits_t sz ~> bits_t sz ~> bits_t sz }}
+    | Or sz => {{ bits_t sz ~> bits_t sz ~> bits_t sz }}
+    | Not sz => {{ bits_t sz ~> bits_t 0 ~> bits_t sz }}
+    | Lsl bits_sz shift_sz => {{ bits_t bits_sz ~> bits_t shift_sz ~> bits_t bits_sz }}
+    | Lsr bits_sz shift_sz => {{ bits_t bits_sz ~> bits_t shift_sz ~> bits_t bits_sz }}
+    | Eq sz => {{ bits_t sz ~> bits_t sz ~> bits_t 1 }}
+    | Concat sz1 sz2 => {{ bits_t sz1 ~> bits_t sz2 ~> bits_t (sz1 + sz2) }}
+    | UIntPlus sz => {{ bits_t sz ~> bits_t sz ~> bits_t sz }}
+    | ZExtL sz nzeroes => {{ bits_t sz ~> bits_t 0 ~> bits_t (nzeroes + sz) }}
+    | ZExtR sz nzeroes => {{ bits_t sz ~> bits_t 0 ~> bits_t (sz + nzeroes) }}
+    end
+  | @StructFn fn sig idx =>
+    {{ struct_t sig ~> bits_t 0 ~> snd (Vector_nth sig.(sv_data) idx) }}
+  end.
+
 Definition prim_sel {sz} (bs: bits sz) (idx: bits (log2 sz)) :=
   match Bits.to_index sz idx with
   | Some idx => Bits.nth bs idx
@@ -51,54 +135,54 @@ Definition prim_sel {sz} (bs: bits sz) (idx: bits (log2 sz)) :=
 Definition prim_uint_plus {sz} (bs1 bs2: bits sz) :=
   Bits.of_N sz (Bits.to_N bs1 + Bits.to_N bs2)%N.
 
-Definition prim_uSigma (fn: prim_ufn_t) '(bits_t sz1) '(bits_t sz2): prim_fn_t :=
-  match fn with
-  | USel => Sel sz1
-  | UPart width => Part sz1 width
-  | UAnd => And sz1
-  | UOr => Or sz1
-  | UNot => Not sz1
-  | ULsl => Lsl sz1 sz2
-  | ULsr => Lsr sz1 sz2
-  | UEq => Eq sz1
-  | UConcat => Concat sz1 sz2
-  | UUIntPlus => UIntPlus sz1
-  | UZExtL nzeroes => ZExtL sz1 nzeroes
-  | UZExtR nzeroes => ZExtR sz1 nzeroes
+(* Record struct_field_selector {fields: struct_sig} := *)
+(*   { sfs_field_name : string; *)
+(*     sfs_field_type : type; *)
+(*     sfs_correct : member (sfs_field_name, sfs_field_type) fields }. *)
+(* Arguments struct_field_selector : clear implicits. *)
+
+Fixpoint member_map {K K': Type} (f: K -> K') (k: K) (ls: list K)
+         (m: member k ls) : member (f k) (List.map f ls) :=
+  match m in (member k ls) return (member (f k) (List.map f ls)) with
+  | MemberHd k sig =>
+    MemberHd (f k) (List.map f sig)
+  | MemberTl k k' sig m' =>
+    MemberTl (f k) (f k') (List.map f sig) (member_map f k sig m')
   end.
 
-(* Require Import Coq.Lists.List. *)
-(* Import ListNotations. *)
-(* Compute (List.map (fun x => (x, Nat.log2 x, log2 x)) [0;1;2;3;4;5;6;7;8;9;10;11;12;13;14;15;16;17;18;19;20;21;22;23;24;25;26;27;28;29;30;31;32;33;34]). *)
+Require Import SGA.Vect.
+Fixpoint list_nth_index {K: Type} (l: list K) (idx: index (List.length l)) {struct l} : K.
+  destruct l; destruct idx.
+  - exact k.
+  - exact (list_nth_index K l a).
+Defined.
 
-Definition prim_Sigma (fn: prim_fn_t) : ExternalSignature :=
-  match fn with
-  | Sel sz => {{ sz ~> log2 sz ~> 1 }}
-  | Part sz width => {{ sz ~> log2 sz ~> width }}
-  | And sz => {{ sz ~> sz ~> sz }}
-  | Or sz => {{ sz ~> sz ~> sz }}
-  | Not sz => {{ sz ~> 0 ~> sz }}
-  | Lsl bits_sz shift_sz => {{ bits_sz ~> shift_sz ~> bits_sz }}
-  | Lsr bits_sz shift_sz => {{ bits_sz ~> shift_sz ~> bits_sz }}
-  | Eq sz => {{ sz ~> sz ~> 1 }}
-  | Concat sz1 sz2 => {{ sz1 ~> sz2 ~> sz1 + sz2 }}
-  | UIntPlus sz => {{ sz ~> sz ~> sz }}
-  | ZExtL sz nzeroes => {{ sz ~> 0 ~> nzeroes + sz }}
-  | ZExtR sz nzeroes => {{ sz ~> 0 ~> sz + nzeroes }}
+Fixpoint type_accessor (tau: type) : Type :=
+  match tau with
+  | bits_t _sz => unit
+  | struct_t fields =>
+    let field_accessors := Vector.map (fun '(k, tau) => type_accessor tau) fields.(sv_data) in
+    { k: index fields.(sv_len) & Vector_nth field_accessors k }
   end.
 
 Definition prim_sigma (fn: prim_fn_t) : prim_Sigma fn :=
   match fn with
-  | Sel _ => fun bs idx => w1 (prim_sel bs idx)
-  | Part _ width => fun base _ => __magic__
-  | And _ => Bits.map2 andb
-  | Or _ => Bits.map2 orb
-  | Not _ => fun bs _ => Bits.map negb bs
-  | Lsl _ _ => fun bs places => Bits.lsl (Bits.to_nat places) bs
-  | Lsr _ _ => fun bs places => Bits.lsr (Bits.to_nat places) bs
-  | Eq sz => fun bs1 bs2 => if eq_dec bs1 bs2 then w1 true else w1 false
-  | UIntPlus _ => fun bs1 bs2 => prim_uint_plus bs1 bs2
-  | Concat _ _ => fun bs1 bs2 => Bits.app bs1 bs2
-  | ZExtL _ nzeroes => fun bs _ => Bits.app (Bits.const nzeroes false) bs
-  | ZExtR _ nzeroes => fun bs _ => Bits.app bs (Bits.const nzeroes false)
+  | BitsFn fn =>
+    match fn with
+    | Sel _ => fun bs idx => w1 (prim_sel bs idx)
+    | Part _ width => fun base _ => __magic__
+    | And _ => Bits.map2 andb
+    | Or _ => Bits.map2 orb
+    | Not _ => fun bs _ => Bits.map negb bs
+    | Lsl _ _ => fun bs places => Bits.lsl (Bits.to_nat places) bs
+    | Lsr _ _ => fun bs places => Bits.lsr (Bits.to_nat places) bs
+    | Eq sz => fun bs1 bs2 => if eq_dec bs1 bs2 then w1 true else w1 false
+    | UIntPlus _ => fun bs1 bs2 => prim_uint_plus bs1 bs2
+    | Concat _ _ => fun bs1 bs2 => Bits.app bs1 bs2
+    | ZExtL _ nzeroes => fun bs _ => Bits.app (Bits.const nzeroes false) bs
+    | ZExtR _ nzeroes => fun bs _ => Bits.app bs (Bits.const nzeroes false)
+    end
+  | StructFn Init sig m => fun s _ => __magic__
+  | StructFn Get sig m => fun s _ => __magic__
+  | StructFn Put sig m => fun s _ => __magic__
   end.
