Types.v
@@ -1,24 +1,44 @@
-Require Import SGA.Vect.
+Require Export SGA.Common SGA.Vect.
+Require Export Coq.Strings.String.
+Require Import Coq.Vectors.Vector.
 
-Inductive type :=
-| bits_t (n: nat).
+Record struct_sig' {A} :=
+  { sv_len: nat;
+    sv_name: string;
+    sv_data: Vector.t (string * A) sv_len }.
+Arguments struct_sig' : clear implicits.
 
-Coercion Nat_of_type '(bits_t n) :=
-  n.
+Inductive type : Type :=
+| bits_t (sz: nat)
+| struct_t (sig: struct_sig' type).
 
-Coercion Type_of_type (tau: type) :=
-  bits tau.
+Notation struct_sig := (struct_sig' type).
+
+Fixpoint type_sz tau :=
+  match tau with
+  | bits_t sz => sz
+  | struct_t fields => Vector.fold_left (fun acc '(_, tau') => acc + type_sz tau') 0 fields.(sv_data)
+  end.
+
+Coercion type_sz : type >-> nat.
+
+Fixpoint type_denote tau : Type :=
+  match tau with
+  | bits_t sz => bits sz
+  | struct_t fields =>
+    Vector.fold_left (fun acc '(_, tau) => type_denote tau * acc)%type unit fields.(sv_data)
+  end.
+
+Coercion type_denote : type >-> Sortclass.
 
 Record ExternalSignature :=
-  FunSig { arg1Type: type;
-           arg2Type: type;
-           retType: type }.
+  FunSig { arg1Type: type; arg2Type: type; retType: type }.
 
 Notation "{{ a1 ~> a2 ~> ret }}" :=
-  {| arg1Type := bits_t a1; arg2Type := bits_t a2; retType := bits_t ret |}
+  {| arg1Type := a1; arg2Type := a2; retType := ret |}
     (at level 200, no associativity).
 
-Coercion Type_of_signature fn :=
+Coercion ExternalSignature_denote fn :=
   fn.(arg1Type) -> fn.(arg2Type) -> fn.(retType).
 
 Lemma ExternalSignature_injRet :
@@ -27,3 +47,15 @@ Lemma ExternalSignature_injRet :
     FunSig s1' s2' retType' ->
     retType = retType'.
 Proof. now inversion 1. Qed.
+
+Inductive type_kind := kind_bits | kind_struct {len: nat} (sig: struct_sig).
+
+Inductive fn_tc_error :=
+| kind_mismatch (expected: type_kind)
+| unbound_field (f: string) (sig: struct_sig).
+
+Definition assert_bits_t (tau: type) : result nat fn_tc_error :=
+  match tau with
+  | bits_t sz => Success sz
+  | struct_t _ => Failure (kind_mismatch kind_bits)
+  end.
