Interop.v
@@ -2,126 +2,127 @@ Require Import Coq.Strings.String.
 Require Import SGA.Environments SGA.Types SGA.Circuits SGA.Primitives.
 
 Section Interop.
-  Inductive interop_ufn_t {custom_fn_t: Type} :=
-  | UPrimFn (fn: prim_ufn_t)
-  | UCustomFn (fn: custom_fn_t).
+  Context {custom_ufn_t custom_fn_t: Type}.
 
-  Inductive interop_fn_t {custom_fn_t: Type} :=
+  Inductive interop_ufn_t :=
+  | UPrimFn (fn: prim_ufn_t)
+  | UCustomFn (fn: custom_ufn_t).
+
+  Inductive interop_fn_t :=
   | PrimFn (fn: prim_fn_t)
   | CustomFn (fn: custom_fn_t).
 
   Definition interop_Sigma
-             {fn_t}
-             (Sigma: fn_t -> ExternalSignature)
-    : @interop_fn_t fn_t -> ExternalSignature  :=
+             (Sigma: custom_fn_t -> ExternalSignature)
+    : interop_fn_t -> ExternalSignature  :=
     fun fn => match fn with
            | PrimFn fn => prim_Sigma fn
            | CustomFn fn => Sigma fn
            end.
 
   Definition interop_uSigma
-             {ufn_t fn_t}
-             (uSigma: ufn_t -> type -> type -> fn_t)
-             (fn: @interop_ufn_t ufn_t)
+             (uSigma: custom_ufn_t -> type -> type -> result custom_fn_t fn_tc_error)
+             (fn: interop_ufn_t)
              (tau1 tau2: type)
-    : @interop_fn_t fn_t  :=
+    : result interop_fn_t fn_tc_error :=
     match fn with
-    | UPrimFn fn => PrimFn (prim_uSigma fn tau1 tau2)
-    | UCustomFn fn => CustomFn (uSigma fn tau1 tau2)
+    | UPrimFn fn => let/res fn := prim_uSigma fn tau1 tau2 in
+                   Success (PrimFn fn)
+    | UCustomFn fn => let/res fn := uSigma fn tau1 tau2 in
+                     Success (CustomFn fn)
     end.
 
   Definition interop_sigma
-             {fn_t}
-             {Sigma: fn_t -> ExternalSignature}
-             (sigma: forall fn: fn_t, Sigma fn)
-    : forall fn: @interop_fn_t fn_t, interop_Sigma Sigma fn :=
+             {Sigma: custom_fn_t -> ExternalSignature}
+             (sigma: forall fn: custom_fn_t, Sigma fn)
+    : forall fn: interop_fn_t, interop_Sigma Sigma fn :=
     fun fn => match fn with
            | PrimFn fn => prim_sigma fn
            | CustomFn fn => sigma fn
            end.
-
-  Inductive interop_empty_t :=.
-  Definition interop_empty_Sigma (fn: interop_empty_t)
-    : ExternalSignature := match fn with end.
-  Definition interop_empty_uSigma (fn: interop_empty_t) (_ _: type)
-    : interop_empty_t := match fn with end.
-  Definition interop_empty_sigma fn
-    : interop_empty_Sigma fn := match fn with end.
-
-  Record sga_package_t :=
-    { (** [sga_reg_t]: The type of variables used in let bindings.
-          Typically [string]. *)
-      sga_var_t: Type;
-      (** [sga_var_names]: These names are used to generate readable code. *)
-      sga_var_names: sga_var_t -> string;
-
-      (** [sga_reg_t]: The type of registers used in the program.
-          Typically an inductive [R0 | R1 | …] *)
-      sga_reg_t: Type;
-      (** [sga_reg_names]: These names are used to generate readable code. *)
-      sga_reg_names: sga_reg_t -> string;
-      (** [sga_reg_types]: The type of data stored in each register. *)
-      sga_reg_types: sga_reg_t -> type;
-      (** [sga_reg_types]: The type of data stored in each register. *)
-      sga_reg_init: forall r: sga_reg_t, sga_reg_types r;
-      (** [sga_reg_finite]: We need to be able to enumerate the set of registers
-          that the program uses. *)
-      sga_reg_finite: FiniteType sga_reg_t;
-
-      (** [sga_custom_fn_t]: The type of custom functions used in the program.
-          The [fn_t] used by the program itself should be [interop_fn_t
-          sga_custom_fn_t], so the program can call primitives using (PrimFn …)
-          and custom functions using (CustomFn …). *)
-      sga_custom_fn_t: Type;
-      (** [sga_custom_fn_t]: The signature of each function. *)
-      sga_custom_fn_types: forall fn: sga_custom_fn_t, ExternalSignature;
-      (** [sga_custom_fn_names]: These names are used to generate readable code. *)
-      sga_custom_fn_names: forall fn: sga_custom_fn_t, string;
-
-      (** [sga_rule_name_t]: The type of rule names.
-          Typically an inductive [rule1 | rule2 | …]. **)
-      sga_rule_name_t: Type;
-      (** [sga_rules]: The rules of the program. **)
-      sga_rules: forall _: sga_rule_name_t,
-          TypedSyntax.rule sga_var_t sga_reg_types (interop_Sigma sga_custom_fn_types);
-      (** [sga_rule_names]: These names are used to generate readable code. **)
-      sga_rule_names: sga_rule_name_t -> string;
-
-      (** [sga_scheduler]: The scheduler. **)
-      sga_scheduler: TypedSyntax.scheduler sga_rule_name_t;
-
-      (** [sga_module_name]: The name of the module to compile. **)
-      sga_module_name: string
-    }.
-
-  Record circuit_package_t :=
-    { cp_prog: sga_package_t;
-
-      (** [cp_reg_env]: This describes how the program concretely stores maps
-          keyed by registers (this is used in the type of [cp_circuit], which is
-          essentially a list of circuits, one per register. *)
-      cp_reg_Env: Env cp_prog.(sga_reg_t);
-
-      (** [cp_circuit]: The actual circuit scheduler circuit generated by the
-          compiler (really a list of circuits, one per register).  This should
-          use [interop_fn_t cp_custom_fn_t] as the function type (and
-          [interop_fn_Sigma cp_custom_fn_types] as the environment of
-          signatures). *)
-      cp_circuit: @state_transition_circuit
-                    (cp_prog.(sga_reg_t)) (@interop_fn_t cp_prog.(sga_custom_fn_t))
-                    (cp_prog.(sga_reg_types)) (interop_Sigma cp_prog.(sga_custom_fn_types))
-                    cp_reg_Env;
-    }.
-
-  Definition compile_sga_package (s: sga_package_t) : circuit_package_t :=
-    let FT := s.(sga_reg_finite) in
-    {| cp_prog := s;
-       cp_circuit :=
-         let R := s.(sga_reg_types) in
-         let Sigma := interop_Sigma s.(sga_custom_fn_types) in
-         let r := ContextEnv.(create) (readRegisters R Sigma) in
-         compile_scheduler r s.(sga_rules) s.(sga_scheduler) |}.
 End Interop.
+
+Inductive interop_empty_t :=.
+Definition interop_empty_Sigma (fn: interop_empty_t)
+  : ExternalSignature := match fn with end.
+Definition interop_empty_uSigma (fn: interop_empty_t) (_ _: type)
+  : result interop_empty_t fn_tc_error := match fn with end.
+Definition interop_empty_sigma fn
+  : interop_empty_Sigma fn := match fn with end.
+
+Record sga_package_t :=
+  { (** [sga_reg_t]: The type of variables used in let bindings.
+        Typically [string]. *)
+    sga_var_t: Type;
+    (** [sga_var_names]: These names are used to generate readable code. *)
+    sga_var_names: sga_var_t -> string;
+
+    (** [sga_reg_t]: The type of registers used in the program.
+        Typically an inductive [R0 | R1 | …] *)
+    sga_reg_t: Type;
+    (** [sga_reg_names]: These names are used to generate readable code. *)
+    sga_reg_names: sga_reg_t -> string;
+    (** [sga_reg_types]: The type of data stored in each register. *)
+    sga_reg_types: sga_reg_t -> type;
+    (** [sga_reg_types]: The type of data stored in each register. *)
+    sga_reg_init: forall r: sga_reg_t, sga_reg_types r;
+    (** [sga_reg_finite]: We need to be able to enumerate the set of registers
+          that the program uses. *)
+    sga_reg_finite: FiniteType sga_reg_t;
+
+    (** [sga_custom_fn_t]: The type of custom functions used in the program.
+        The [fn_t] used by the program itself should be [interop_fn_t
+        sga_custom_fn_t], so the program can call primitives using (PrimFn …)
+        and custom functions using (CustomFn …). *)
+    sga_custom_fn_t: Type;
+    (** [sga_custom_fn_t]: The signature of each function. *)
+    sga_custom_fn_types: forall fn: sga_custom_fn_t, ExternalSignature;
+    (** [sga_custom_fn_names]: These names are used to generate readable code. *)
+    sga_custom_fn_names: forall fn: sga_custom_fn_t, string;
+
+    (** [sga_rule_name_t]: The type of rule names.
+        Typically an inductive [rule1 | rule2 | …]. **)
+    sga_rule_name_t: Type;
+    (** [sga_rules]: The rules of the program. **)
+    sga_rules: forall _: sga_rule_name_t,
+        TypedSyntax.rule sga_var_t sga_reg_types (interop_Sigma sga_custom_fn_types);
+    (** [sga_rule_names]: These names are used to generate readable code. **)
+    sga_rule_names: sga_rule_name_t -> string;
+
+    (** [sga_scheduler]: The scheduler. **)
+    sga_scheduler: TypedSyntax.scheduler sga_rule_name_t;
+
+    (** [sga_module_name]: The name of the module to compile. **)
+    sga_module_name: string
+  }.
+
+Record circuit_package_t :=
+  { cp_prog: sga_package_t;
+
+    (** [cp_reg_env]: This describes how the program concretely stores maps
+        keyed by registers (this is used in the type of [cp_circuit], which is
+        essentially a list of circuits, one per register. *)
+    cp_reg_Env: Env cp_prog.(sga_reg_t);
+
+    (** [cp_circuit]: The actual circuit scheduler circuit generated by the
+        compiler (really a list of circuits, one per register).  This should
+        use [interop_fn_t cp_custom_fn_t] as the function type (and
+        [interop_fn_Sigma cp_custom_fn_types] as the environment of
+        signatures). *)
+    cp_circuit: @state_transition_circuit
+                  (cp_prog.(sga_reg_t)) (@interop_fn_t cp_prog.(sga_custom_fn_t))
+                  (cp_prog.(sga_reg_types)) (interop_Sigma cp_prog.(sga_custom_fn_types))
+                  cp_reg_Env;
+  }.
+
+Definition compile_sga_package (s: sga_package_t) : circuit_package_t :=
+  let FT := s.(sga_reg_finite) in
+  {| cp_prog := s;
+     cp_circuit :=
+       let R := s.(sga_reg_types) in
+       let Sigma := interop_Sigma s.(sga_custom_fn_types) in
+       let r := ContextEnv.(create) (readRegisters R Sigma) in
+       compile_scheduler r s.(sga_rules) s.(sga_scheduler) |}.
 
 Arguments interop_fn_t: clear implicits.
 Arguments interop_ufn_t: clear implicits.
